---
layout: post
title:  class 6 Chapter 3.3 Binomial Theorem
date:   2017-01-23 11:00:05
categories: Graph_Theory_note
tags: intro binomial_theorem 
---

*content
{: toc}

## "N-nomials"
Bionomial "look like" $$1-2x+12x^{3}+x^{17}$$

Monomial  $$-4x^{6}$$

bionomial $$1+x$$






What do binomial coefs have to do with binomials?

## Binomial Theorem

$$(1+x)^{n}= \sum_{k=0}^{n}\binom{n}{k}x^{k}$$

Pf1: Induction, with pascal's triangle identity (homework)

pf2: 

$$(1+x) \cdot (1+x) \cdot (1+x) \cdot (1+x) \cdot .... (1+x)$$

gives $$2^{n}$$ summands

as each factor contribute either 1 or x (2 possibilities)

How many summands have exactly k x's?

choose k of the factors to contribute an x, $$\binom{n}{k}$$ in number. 



<div style="text-align: right"> Q.E.D</div>

Prop i  $$\sum_{k=0}^n \binom{n}{k} = 2^{n}$$

### proof 1: 

RHS is # subset of a set w/n eHs

LHS is # subets 

satistified by size(bijection)


### proof 2: 

$$(1+1)^{n} = \sum_{k=0}^{n} \binom{n}{k} 1^{k}$$



prop: If n≥0, then $$\sum(-1)^{k}\binom{n}{k}=0$$

same # of even-sized subsets as # odd_size of a finite set,)

If n is odd, obvious

for n = 3

1-3+3-1

for n = 5

1-5+10-10+5-1

prop: if n ≥ 0, then 

$$\sum_{k=0}^{n} \binom{n}{k}^{2}=\binom{2n}{n}$$

(see textbook for bijection proof)

proof 

notice $$ \binom{2n}{n}$$ is coefficient 

of $$x^{n} \ in \ (1+n)^{2n}$$

then 

$$(1+x)^{2n} = ((1+x)^{n})^{2}$$

$$= (\sum_{k=0}^{n}\binom{n}{k}x^{k})^{2}$$

$$=\sum_{k=0}^{n}\binom{n}{k} \cdot \binom{n}{n-k}$$

by lemma 1

$$\binom{n}{n-k}=\binom{n}{k}$$


